abs1_comb_thm/abs1_comb_hold_ref_rel_tau_drScript.sml
@@ -1,0 +1,177 @@
+open HolKernel bossLib boolLib Parse;
+open wordsLib optionTheory;
+open SPI_stateTheory SPI_relationTheory SPI_tauTheory SPI_return_regsTheory weak_bisimulationTheory;
+open driver_stateTheory driver_relationTheory driver_checkTheory driver_readTheory driver_writeTheory;
+open ds_abs1_stateTheory ds_abs1_relTheory ds_abs1_rxTheory ds_abs1_xferTheory;
+open ref_relTheory board_memTheory;
+
+val _ = new_theory "abs1_comb_hold_ref_rel_tau_dr";
+
+(* theorems related to rx automaton *)
+(* ref_rel holds if ds_abs1 has tau_dr transition and ds_abs1.state = abs1_rx_ready *)
+val ref_rel_holds_tau_dr_abs1_rx_ready = store_thm("ref_rel_holds_tau_dr_abs1_rx_ready",
+``!spi dr ds_abs1.
+(ref_rel ds_abs1 (dr,spi)) /\ (ds_abs1.state = abs1_rx_ready) /\ 
+(IS_STATE_REL ds_abs1 dr spi) ==>
+(?dr' spi'. local_tr (dr,spi) tau (dr',spi') /\
+ref_rel (driver_abs1_rx_operations ds_abs1) (dr',spi')) \/
+(?n dr' spi'. n_tau_tr n local_tr (dr,spi) tau (dr',spi') /\
+ref_rel (driver_abs1_rx_operations ds_abs1) (dr',spi'))``,
+rw [driver_abs1_rx_operations_def] >>
+`dr.dr_rx.rx_left_length = ds_abs1.ds_abs1_rx.rx_left_length` by fs [ref_rel_def] >>
+`(dr.state = dr_rx_check_rxs /\ spi.state = rx_data_ready) \/
+(dr.state = dr_rx_read_rxs /\ spi.state = rx_data_ready)` by fs [IS_STATE_REL_def] >|
+[(* dr_rx_check_rxs and rx_data_ready *)
+`dr.dr_last_read_ad = SOME SPI0_CH0STAT /\ ?v. dr.dr_last_read_v =  SOME v` by fs [ref_rel_def] >>
+Cases_on `(0 >< 0) v:word1 = 1w` >|
+[(* the stored value of rxs is 1w *)
+DISJ1_TAC >>
+rw [local_tr_cases, driver_tr_cases, DR_TAU_ENABLE_def] >>
+Q.EXISTS_TAC `dr_check dr SPI0_CH0STAT (THE dr.dr_last_read_v)` >> 
+Q.EXISTS_TAC `spi` >>
+rw [dr_check_def, dr_check_rx_ch0stat_def, driver_abs1_rx_ready_op_def] >>
+fs [ref_rel_def, IS_STATE_REL_def], 
+(* the stored value of rxs is 0w *)
+DISJ2_TAC >>
+Q.EXISTS_TAC `SUC 1:num` >>
+rw [n_tau_tr_def, n_tau_tr_SUC, local_tr_cases, driver_tr_cases, spi_tr_cases,
+DR_TAU_ENABLE_def, SPI_TAU_ENABLE_def, DR_WR_ENABLE_def, DR_RD_ENABLE_def] >>
+`dr_check dr SPI0_CH0STAT v = dr with state := dr_rx_read_rxs` 
+by rw [dr_check_def, dr_check_rx_ch0stat_def] >>
+rw [] >>
+`dr_read (dr with state := dr_rx_read_rxs) = dr with <| state := dr_rx_check_rxs; 
+dr_last_read_ad := SOME SPI0_CH0STAT |>` by rw [dr_read_def, dr_read_ch0stat_def] >>
+rw [] >>
+Q.EXISTS_TAC `dr_check (dr with <| state := dr_rx_check_rxs; 
+dr_last_read_ad := SOME SPI0_CH0STAT;
+dr_last_read_v := SOME (read_SPI_regs_value SPI0_CH0STAT spi) |>) 
+SPI0_CH0STAT (read_SPI_regs_value SPI0_CH0STAT spi)` >>
+Q.EXISTS_TAC `read_SPI_regs_state SPI0_CH0STAT spi` >>
+rw [read_SPI_regs_state_def, read_SPI_regs_value_def, read_SPI_regs_def, SPI0_CH0STAT_def,
+SPI0_PA_RANGE_def, SPI0_START_def, SPI0_END_def, SPI0_SYSCONFIG_def, SPI0_SYSSTATUS_def,
+SPI0_MODULCTRL_def, SPI0_CH0CONF_def] >>
+`spi.regs.CH0STAT.RXS = 1w` by fs [ref_rel_def] >>
+rw [dr_check_def, dr_check_rx_ch0stat_def, build_CH0STAT_def, SPI0_CH0STAT_def, 
+driver_abs1_rx_ready_op_def] >>
+fs [ref_rel_def, IS_STATE_REL_def] >>
+FULL_SIMP_TAC (std_ss++WORD_ss++WORD_EXTRACT_ss) []],
+(* dr_rx_read_rxs and rx_data_ready *)
+DISJ2_TAC >>
+Q.EXISTS_TAC `SUC 0` >>
+rw [n_tau_tr_def, local_tr_cases, driver_tr_cases, spi_tr_cases, 
+DR_RD_ENABLE_def, DR_WR_ENABLE_def, DR_TAU_ENABLE_def, SPI_TAU_ENABLE_def] >>
+`dr_read dr = dr with <| state := dr_rx_check_rxs; 
+dr_last_read_ad := SOME SPI0_CH0STAT |>` by rw [dr_read_def, dr_read_ch0stat_def] >>
+rw [] >>
+Q.EXISTS_TAC `dr_check (dr with <| state := dr_rx_check_rxs; 
+dr_last_read_ad := SOME SPI0_CH0STAT;
+dr_last_read_v := SOME (read_SPI_regs_value SPI0_CH0STAT spi) |>) 
+SPI0_CH0STAT (read_SPI_regs_value SPI0_CH0STAT spi)` >>
+Q.EXISTS_TAC `read_SPI_regs_state SPI0_CH0STAT spi` >>
+rw [read_SPI_regs_state_def, read_SPI_regs_value_def, read_SPI_regs_def, SPI0_CH0STAT_def,
+SPI0_PA_RANGE_def, SPI0_START_def, SPI0_END_def, SPI0_SYSCONFIG_def, SPI0_SYSSTATUS_def,
+SPI0_MODULCTRL_def, SPI0_CH0CONF_def] >>
+`spi.regs.CH0STAT.RXS = 1w` by fs [ref_rel_def] >>
+rw [dr_check_def, dr_check_rx_ch0stat_def, build_CH0STAT_def, SPI0_CH0STAT_def, 
+driver_abs1_rx_ready_op_def] >>
+fs [ref_rel_def, IS_STATE_REL_def] >>
+FULL_SIMP_TAC (std_ss++WORD_ss++WORD_EXTRACT_ss) []]);
+
+(* ref_rel holds if ds_abs1 has tau_dr transition and ds_abs1.state = abs1_rx_fetch_data *)
+val ref_rel_holds_tau_dr_abs1_rx_fetch_data = store_thm("ref_rel_holds_tau_dr_abs1_rx_fetch_data",
+``!spi dr ds_abs1.
+(ref_rel ds_abs1 (dr,spi)) /\ (ds_abs1.state = abs1_rx_fetch_data) /\ 
+(IS_STATE_REL ds_abs1 dr spi) ==>
+?dr' spi'. local_tr (dr,spi) tau (dr',spi') /\
+ref_rel (driver_abs1_rx_operations ds_abs1) (dr',spi')``,
+rw [driver_abs1_rx_operations_def, driver_abs1_rx_fetch_data_op_def] >>
+`dr.state = dr_rx_fetch_data /\ spi.state = rx_receive_data` by fs [IS_STATE_REL_def] >>
+`dr.dr_last_read_ad = SOME SPI0_RX0 /\ ?v. dr.dr_last_read_v =  SOME v` by fs [ref_rel_def] >>
+rw [local_tr_cases, driver_tr_cases, DR_TAU_ENABLE_def] >>
+Q.EXISTS_TAC `dr_check dr SPI0_RX0 (THE dr.dr_last_read_v)` >> 
+Q.EXISTS_TAC `spi` >>
+rw [dr_check_def, dr_check_rx0_def] >>
+fs [ref_rel_def, IS_STATE_REL_def]);
+
+(* ref_rel holds if ds_abs1 has tau_dr transition and ds_abs1.state = abs1_rx_next *)
+val ref_rel_holds_tau_dr_abs1_rx_next = store_thm("ref_rel_holds_tau_dr_abs1_rx_next",
+``!spi dr ds_abs1.
+(ref_rel ds_abs1 (dr,spi)) /\ (ds_abs1.state = abs1_rx_next) /\ 
+(IS_STATE_REL ds_abs1 dr spi) ==>
+?dr' spi'. local_tr (dr,spi) tau (dr',spi') /\
+ref_rel (driver_abs1_rx_operations ds_abs1) (dr',spi')``,
+rw [driver_abs1_rx_operations_def, driver_abs1_rx_next_op_def] >>
+`dr.state = dr_rx_fetch_data /\ spi.state = rx_update_RX0` by fs [IS_STATE_REL_def] >>
+`dr.dr_last_read_ad = SOME SPI0_RX0 /\ ?v. dr.dr_last_read_v =  SOME v` by fs [ref_rel_def] >>
+rw [local_tr_cases, driver_tr_cases, DR_TAU_ENABLE_def] >>
+Q.EXISTS_TAC `dr_check dr SPI0_RX0 (THE dr.dr_last_read_v)` >> 
+Q.EXISTS_TAC `spi` >>
+rw [dr_check_def, dr_check_rx0_def] >>
+fs [ref_rel_def, IS_STATE_REL_def]);
+
+(* ref_rel holds if ds_abs1 has tau_dr transition and ds_abs1.state = abs1_rx_next_ready *)
+val ref_rel_holds_tau_dr_abs1_rx_next_ready = store_thm("ref_rel_holds_tau_dr_abs1_rx_next_ready",
+``!spi dr ds_abs1.
+(ref_rel ds_abs1 (dr,spi)) /\ (ds_abs1.state = abs1_rx_next_ready) /\ 
+(IS_STATE_REL ds_abs1 dr spi) ==>
+?dr' spi'. local_tr (dr,spi) tau (dr',spi') /\
+ref_rel (driver_abs1_rx_operations ds_abs1) (dr',spi')``,
+rw [driver_abs1_rx_operations_def, driver_abs1_rx_next_ready_op_def] >>
+`dr.state = dr_rx_fetch_data /\ spi.state = rx_data_ready` by fs [IS_STATE_REL_def] >>
+`dr.dr_last_read_ad = SOME SPI0_RX0 /\ ?v. dr.dr_last_read_v =  SOME v` by fs [ref_rel_def] >>
+rw [local_tr_cases, driver_tr_cases, DR_TAU_ENABLE_def] >>
+Q.EXISTS_TAC `dr_check dr SPI0_RX0 (THE dr.dr_last_read_v)` >> 
+Q.EXISTS_TAC `spi` >>
+rw [dr_check_def, dr_check_rx0_def] >>
+fs [ref_rel_def, IS_STATE_REL_def]);
+
+(* (dr',spi') exists for rx *)
+val abs1_comb_hold_ref_rel_tau_dr_rx = 
+store_thm("abs1_comb_hold_ref_rel_tau_dr_rx",
+``!spi dr ds_abs1.
+(ref_rel ds_abs1 (dr,spi)) /\ (DRIVER_ABS1_RX_ENABLE ds_abs1) ==>
+(?dr' spi'. local_tr (dr,spi) tau (dr',spi') /\
+ref_rel (driver_abs1_rx_operations ds_abs1) (dr',spi')) \/
+(?n dr' spi'. n_tau_tr n local_tr (dr,spi) tau (dr',spi') /\
+ref_rel (driver_abs1_rx_operations ds_abs1) (dr',spi'))``,
+rw [DRIVER_ABS1_RX_ENABLE_def] >> 
+`IS_STATE_REL ds_abs1 dr spi` by fs [ref_rel_def] >>
+rw [ref_rel_holds_tau_dr_abs1_rx_ready, ref_rel_holds_tau_dr_abs1_rx_fetch_data,
+ref_rel_holds_tau_dr_abs1_rx_next, ref_rel_holds_tau_dr_abs1_rx_next_ready]);
+
+
+(* theorems related to xfer automaton *)
+(* (dr',spi') exists for xfer *)
+val abs1_comb_hold_ref_rel_tau_dr_xfer = 
+store_thm("abs1_comb_hold_ref_rel_tau_dr_xfer",
+``!spi dr ds_abs1.
+(ref_rel ds_abs1 (dr,spi)) /\ (DRIVER_ABS1_XFER_ENABLE ds_abs1) ==>
+?dr' spi'. local_tr (dr,spi) tau (dr',spi') /\
+ref_rel (driver_abs1_xfer_operations ds_abs1) (dr',spi')``,
+rw [DRIVER_ABS1_XFER_ENABLE_def, driver_abs1_xfer_operations_def,
+driver_abs1_xfer_fetch_data_op_def] >>
+`IS_STATE_REL ds_abs1 dr spi` by fs [ref_rel_def] >>
+`dr.state = dr_xfer_fetch_dataI /\ spi.state = xfer_ready_for_trans` by fs [IS_STATE_REL_def] >>
+`dr.dr_last_read_ad = SOME SPI0_RX0 /\ ?v. dr.dr_last_read_v =  SOME v` by fs [ref_rel_def] >>
+rw [local_tr_cases, driver_tr_cases, DR_TAU_ENABLE_def] >>
+Q.EXISTS_TAC `dr_check dr SPI0_RX0 (THE dr.dr_last_read_v)` >>
+Q.EXISTS_TAC `spi` >>
+rw [] >-
+(`dr.dr_xfer.xfer_cur_length < (LENGTH dr.dr_xfer.xfer_dataOUT_buf)` by fs [ref_rel_def] >>
+rw [dr_check_def, dr_check_rx0_def] >>
+fs [ref_rel_def, IS_STATE_REL_def]) >>
+`~ (dr.dr_xfer.xfer_cur_length < (LENGTH dr.dr_xfer.xfer_dataOUT_buf))` by fs [ref_rel_def] >>
+rw [dr_check_def, dr_check_rx0_def] >>
+fs [ref_rel_def, IS_STATE_REL_def]);
+
+(* simulation: (dr',spi') exists and holds the ref_rel when ds_abs1 has tau_dr transitions *)
+val abs1_comb_hold_ref_rel_tau_dr = 
+store_thm("abs1_comb_hold_ref_rel_tau_dr",
+``!spi dr ds_abs1 ds_abs1'.
+(ref_rel ds_abs1 (dr, spi)) /\ (ds_abs1_dr_tr ds_abs1 tau_dr ds_abs1') ==>
+(?dr' spi'. (local_tr (dr, spi) tau (dr', spi')) /\ (ref_rel ds_abs1' (dr', spi'))) \/
+(?n dr' spi'. (n_tau_tr n local_tr (dr,spi) tau (dr',spi')) /\ (ref_rel ds_abs1' (dr',spi')))``,
+rw [ds_abs1_dr_tr_cases] >>
+rw [abs1_comb_hold_ref_rel_tau_dr_rx, abs1_comb_hold_ref_rel_tau_dr_xfer]);
+
+val _ = export_theory();
