abs1_comb_thm/abs1_comb_hold_ref_rel_tau_spiScript.sml
@@ -1,0 +1,441 @@
+open HolKernel bossLib boolLib Parse;
+open wordsLib;
+open SPI_stateTheory SPI_relationTheory weak_bisimulationTheory SPI_tauTheory SPI_update_regsTheory;
+open driver_stateTheory driver_relationTheory driver_writeTheory driver_readTheory driver_checkTheory;
+open ds_abs1_stateTheory ds_abs1_relTheory ds_abs1_txTheory ds_abs1_rxTheory ds_abs1_xferTheory;
+open ref_relTheory board_memTheory;
+
+val _ = new_theory "abs1_comb_hold_ref_rel_tau_spi";
+
+(* theorems related to tx automaton *)
+(* ref_rel holds if ds_abs1 has tau_spi transition and ds_abs1.state = abs1_tx_idle *)
+val ref_rel_holds_tau_spi_abs1_tx_idle = store_thm("ref_rel_holds_tau_spi_abs1_tx_idle",
+``!spi dr ds_abs1.
+(ref_rel ds_abs1 (dr,spi)) /\ (ds_abs1.state = abs1_tx_idle) /\
+(IS_STATE_REL ds_abs1 dr spi) ==>
+(?dr' spi'. (local_tr (dr, spi) tau (dr', spi')) /\ 
+(ref_rel (spi_abs1_tx_operations ds_abs1) (dr', spi'))) \/
+(?n dr' spi'. (n_tau_tr n local_tr (dr,spi) tau (dr',spi')) /\ 
+(ref_rel (spi_abs1_tx_operations ds_abs1) (dr',spi')))``,
+rw [spi_abs1_tx_operations_def, spi_abs1_tx_idle_op_def] >>
+`(dr.state = dr_tx_read_txs /\ spi.state = tx_channel_enabled) \/
+(dr.state = dr_tx_check_txs /\ spi.state = tx_channel_enabled) \/
+(dr.state = dr_tx_conf_issued /\ spi.state = tx_conf_ready) \/
+(dr.state = dr_tx_idle /\ spi.state = spi_ready)` 
+by fs [IS_STATE_REL_def] >|
+[(* dr_tx_read_txs and tx_channel_enabled *)
+DISJ1_TAC >>
+rw [local_tr_cases, spi_tr_cases, SPI_TAU_ENABLE_def] >>
+EXISTS_TAC ``dr:driver_state`` >>
+EXISTS_TAC ``spi_tau_operations spi:spi_state`` >>
+rw [spi_tau_operations_def, tx_channel_enabled_op_def] >>
+fs [ref_rel_def, IS_STATE_REL_def],
+(* dr_tx_check_txs and tx_channel_enabled *)
+DISJ1_TAC >>
+rw [local_tr_cases, spi_tr_cases, SPI_TAU_ENABLE_def] >>
+EXISTS_TAC ``dr:driver_state`` >>
+EXISTS_TAC ``spi_tau_operations spi:spi_state`` >>
+rw [spi_tau_operations_def, tx_channel_enabled_op_def] >>
+fs [ref_rel_def, IS_STATE_REL_def],
+(* dr_tx_conf_issued and tx_conf_ready *)
+DISJ2_TAC >>
+EXISTS_TAC ``SUC 0:num`` >>
+rw [n_tau_tr_def, local_tr_cases, driver_tr_cases, spi_tr_cases, 
+DR_WR_ENABLE_def, GSYM LEFT_EXISTS_AND_THM] >>
+EXISTS_TAC ``dr_write_state dr: driver_state`` >>
+EXISTS_TAC ``spi_tau_operations (write_SPI_regs (THE (dr_write_address dr)) (THE (dr_write_value dr)) spi)`` >>
+EXISTS_TAC ``(dr_write_state dr, 
+write_SPI_regs (THE (dr_write_address dr)) (THE (dr_write_value dr)) spi)`` >>
+rw [] >|
+[DISJ2_TAC >> 
+DISJ1_TAC >>
+rw [write_SPI_regs_def, dr_write_address_def, dr_write_value_def, dr_write_def, SPI_TAU_ENABLE_def, dr_write_ch0ctrl_def, write_CH0CTRL_def] >>
+fs [SPI0_CH0CTRL_def, SPI0_PA_RANGE_def, SPI0_END_def, SPI0_START_def, SPI0_SYSCONFIG_def, SPI0_MODULCTRL_def, SPI0_CH0CONF_def],
+fs [write_SPI_regs_def, dr_write_address_def, dr_write_value_def, dr_write_state_def, dr_write_def, dr_write_ch0ctrl_def, write_CH0CTRL_def] >>
+rw [SPI0_CH0CTRL_def, SPI0_PA_RANGE_def, SPI0_END_def, SPI0_START_def, SPI0_SYSCONFIG_def, SPI0_MODULCTRL_def, SPI0_CH0CONF_def, spi_tau_operations_def, tx_channel_enabled_op_def] >>
+fs [ref_rel_def, IS_STATE_REL_def]],
+(* dr_tx_idle and spi_ready *)
+DISJ2_TAC >>
+EXISTS_TAC ``SUC 1:num`` >>
+rw [n_tau_tr_def, n_tau_tr_SUC, local_tr_cases, driver_tr_cases, spi_tr_cases,
+DR_WR_ENABLE_def, GSYM LEFT_EXISTS_AND_THM, GSYM RIGHT_EXISTS_AND_THM,
+DR_TAU_ENABLE_def, SPI_TAU_ENABLE_def, DR_RD_ENABLE_def] >>
+rw [dr_write_state_def, dr_write_def, dr_write_ch0conf_tx_def] >>
+`(write_SPI_regs (THE (dr_write_address dr)) (THE (dr_write_value dr)) spi) = 
+spi with <| state := tx_conf_ready; 
+regs := spi.regs with CH0CONF := spi.regs.CH0CONF with
+<|TRM := 2w; FORCE := 1w |> |>` by rw [write_SPI_regs_def, dr_write_address_def, 
+dr_write_value_def, dr_write_def, dr_write_ch0conf_tx_def, write_CH0CONF_comb_def, 
+write_CH0CONF_tx_def, SPI0_CH0CTRL_def, SPI0_PA_RANGE_def, SPI0_END_def, SPI0_START_def,
+SPI0_SYSCONFIG_def, SPI0_MODULCTRL_def, SPI0_CH0CONF_def] >>
+fs [dr_write_ch0ctrl_def] >>
+EXISTS_TAC ``dr with state := dr_tx_read_txs`` >>
+EXISTS_TAC ``spi_tau_operations 
+(write_SPI_regs (THE (dr_write_address (dr with state := dr_tx_conf_issued)))
+(THE (dr_write_value (dr with state := dr_tx_conf_issued)))
+(spi with <| state := tx_conf_ready; regs := spi.regs with CH0CONF := spi.regs.CH0CONF with
+<|TRM := 2w; FORCE := 1w |> |>))`` >>
+rw [] >|
+[DISJ1_TAC >> 
+DISJ2_TAC >> 
+DISJ1_TAC >>
+rw [write_SPI_regs_def, dr_write_address_def, dr_write_value_def, dr_write_def, 
+SPI0_CH0CTRL_def, SPI0_PA_RANGE_def, SPI0_END_def, SPI0_START_def, SPI0_SYSCONFIG_def, 
+SPI0_MODULCTRL_def, SPI0_CH0CONF_def, dr_write_ch0ctrl_def, write_CH0CTRL_def],
+rw [write_SPI_regs_def, dr_write_address_def, dr_write_value_def, dr_write_def, 
+SPI0_CH0CTRL_def, SPI0_PA_RANGE_def, SPI0_END_def, SPI0_START_def, SPI0_SYSCONFIG_def, 
+SPI0_MODULCTRL_def, SPI0_CH0CONF_def, dr_write_ch0ctrl_def] >>
+rw [write_CH0CTRL_def, spi_tau_operations_def, tx_channel_enabled_op_def] >>
+fs [ref_rel_def, IS_STATE_REL_def]]]);
+
+(* ref_rel holds if ds_abs1 has tau_spi transition and ds_abs1.state = abs1_tx_data_1 *)
+val ref_rel_holds_tau_spi_abs1_tx_data_1 = store_thm("ref_rel_holds_tau_spi_abs1_tx_data_1",
+``!spi dr ds_abs1.
+(ref_rel ds_abs1 (dr,spi)) /\ (ds_abs1.state = abs1_tx_data_1) /\
+(IS_STATE_REL ds_abs1 dr spi) ==>
+?dr' spi'. (local_tr (dr, spi) tau (dr', spi')) /\ 
+(ref_rel (spi_abs1_tx_operations ds_abs1) (dr', spi'))``,
+rw [spi_abs1_tx_operations_def, spi_abs1_tx_data_1_op_def] >>
+`(dr.state = dr_tx_read_eot /\ spi.state = tx_trans_data) \/
+(dr.state = dr_tx_check_eot /\ spi.state = tx_trans_data)` by fs [IS_STATE_REL_def] >>
+rw [local_tr_cases, spi_tr_cases, SPI_TAU_ENABLE_def] >>
+EXISTS_TAC ``dr:driver_state`` >>
+EXISTS_TAC ``spi_tau_operations spi:spi_state`` >>
+rw [spi_tau_operations_def, tx_trans_data_op_def] >>
+fs [ref_rel_def, IS_STATE_REL_def]);
+
+(* ref_rel holds if ds_abs1 has tau_spi transition and ds_abs1.state = abs1_tx_data_2 *)
+val ref_rel_holds_tau_spi_abs1_tx_data_2 = store_thm("ref_rel_holds_tau_spi_abs1_tx_data_2",
+``!spi dr ds_abs1.
+(ref_rel ds_abs1 (dr,spi)) /\ (ds_abs1.state = abs1_tx_data_2) /\
+(IS_STATE_REL ds_abs1 dr spi) ==>
+?dr' spi'. (local_tr (dr, spi) tau (dr', spi')) /\ 
+(ref_rel (spi_abs1_tx_operations ds_abs1) (dr', spi'))``,
+rw [spi_abs1_tx_operations_def, spi_abs1_tx_data_2_op_def] >>
+`(dr.state = dr_tx_read_txs /\ spi.state = tx_trans_data) \/
+(dr.state = dr_tx_check_txs /\ spi.state = tx_trans_data)` by fs [IS_STATE_REL_def] >>
+rw [local_tr_cases, spi_tr_cases, SPI_TAU_ENABLE_def] >>
+EXISTS_TAC ``dr:driver_state`` >>
+EXISTS_TAC ``spi_tau_operations spi:spi_state`` >>
+rw [spi_tau_operations_def, tx_trans_data_op_def] >>
+fs [ref_rel_def, IS_STATE_REL_def]);
+
+(* ref_rel holds if ds_abs1 has tau_spi transition and ds_abs1.state = abs1_tx_update *)
+val ref_rel_holds_tau_spi_abs1_tx_update = store_thm("ref_rel_holds_tau_spi_abs1_tx_update",
+``!spi dr ds_abs1.
+(ref_rel ds_abs1 (dr,spi)) /\ (ds_abs1.state = abs1_tx_update) /\
+(IS_STATE_REL ds_abs1 dr spi) ==>
+?dr' spi'. (local_tr (dr, spi) tau (dr', spi')) /\ 
+(ref_rel (spi_abs1_tx_operations ds_abs1) (dr', spi'))``,
+rw [spi_abs1_tx_operations_def, spi_abs1_tx_update_op_def] >>
+`(dr.state = dr_tx_read_txs /\ spi.state = tx_trans_update) \/
+(dr.state = dr_tx_check_txs /\ spi.state = tx_trans_update)` by fs [IS_STATE_REL_def] >>
+rw [local_tr_cases, spi_tr_cases, SPI_TAU_ENABLE_def] >>
+EXISTS_TAC ``dr:driver_state`` >>
+EXISTS_TAC ``spi_tau_operations spi:spi_state`` >>
+rw [spi_tau_operations_def, tx_trans_update_op_def] >>
+fs [ref_rel_def, IS_STATE_REL_def]);
+
+(* ref_rel holds if ds_abs1 has tau_spi transition and ds_abs1.state = abs1_tx_update *)
+val ref_rel_holds_tau_spi_abs1_tx_last_update = store_thm("ref_rel_holds_tau_spi_abs1_tx_last_update",
+``!spi dr ds_abs1.
+(ref_rel ds_abs1 (dr,spi)) /\ (ds_abs1.state = abs1_tx_last_update) /\
+(IS_STATE_REL ds_abs1 dr spi) ==>
+?dr' spi'. (local_tr (dr, spi) tau (dr', spi')) /\ 
+(ref_rel (spi_abs1_tx_operations ds_abs1) (dr', spi'))``,
+rw [spi_abs1_tx_operations_def, spi_abs1_tx_last_update_op_def] >>
+`(dr.state = dr_tx_read_eot /\ spi.state = tx_trans_update) \/
+(dr.state = dr_tx_check_eot /\ spi.state = tx_trans_update)` by fs [IS_STATE_REL_def] >>
+rw [local_tr_cases, spi_tr_cases, SPI_TAU_ENABLE_def] >>
+EXISTS_TAC ``dr:driver_state`` >>
+EXISTS_TAC ``spi_tau_operations spi:spi_state`` >>
+rw [spi_tau_operations_def, tx_trans_update_op_def] >>
+fs [ref_rel_def, IS_STATE_REL_def]);
+
+(* (dr',spi') exists for tx automaton *)
+val abs1_comb_hold_ref_rel_tau_spi_tx = store_thm("abs1_comb_hold_ref_rel_tau_spi_tx",
+``!spi dr ds_abs1.
+(ref_rel ds_abs1 (dr, spi)) /\ (SPI_ABS1_TX_ENABLE ds_abs1) ==>
+(?dr' spi'. (local_tr (dr, spi) tau (dr', spi')) /\ 
+(ref_rel (spi_abs1_tx_operations ds_abs1) (dr', spi'))) \/
+(?n dr' spi'. (n_tau_tr n local_tr (dr,spi) tau (dr',spi')) /\ 
+(ref_rel (spi_abs1_tx_operations ds_abs1) (dr',spi')))``,
+rw [SPI_ABS1_TX_ENABLE_def] >>
+`IS_STATE_REL ds_abs1 dr spi` by fs [ref_rel_def] >>
+rw [ref_rel_holds_tau_spi_abs1_tx_idle, ref_rel_holds_tau_spi_abs1_tx_data_1,
+ref_rel_holds_tau_spi_abs1_tx_data_2, ref_rel_holds_tau_spi_abs1_tx_update,
+ref_rel_holds_tau_spi_abs1_tx_last_update]);
+
+
+(* theorems related to rx automaton *)
+(* ref_rel holds if ds_abs1 performs tau_spi transition and ds_abs1.state = abs1_rx_idle *)
+val ref_rel_holds_tau_spi_abs1_rx_idle = store_thm("ref_rel_holds_tau_spi_abs1_rx_idle",
+``!spi dr ds_abs1.
+(ref_rel ds_abs1 (dr,spi)) /\ (ds_abs1.state = abs1_rx_idle) /\
+(IS_STATE_REL ds_abs1 dr spi) ==>
+(?dr' spi'. (local_tr (dr, spi) tau (dr', spi')) /\ 
+(ref_rel (spi_abs1_rx_operations ds_abs1) (dr', spi'))) \/
+(?n dr' spi'. (n_tau_tr n local_tr (dr,spi) tau (dr',spi')) /\ 
+(ref_rel (spi_abs1_rx_operations ds_abs1) (dr',spi')))``,
+rw [spi_abs1_rx_operations_def, spi_abs1_rx_idle_op_def] >>
+`(dr.state = dr_rx_read_rxs /\ spi.state = rx_channel_enabled) \/
+(dr.state = dr_rx_check_rxs /\ spi.state = rx_channel_enabled) \/
+(dr.state = dr_rx_conf_issued /\ spi.state = rx_conf_ready) \/
+(dr.state = dr_rx_idle /\ spi.state = spi_ready)` by fs [IS_STATE_REL_def] >|
+[(* dr_rx_read_rxs and rx_channel_enabled *)
+DISJ1_TAC >>
+rw [local_tr_cases, spi_tr_cases, SPI_TAU_ENABLE_def] >>
+EXISTS_TAC ``dr:driver_state`` >>
+EXISTS_TAC ``spi_tau_operations spi:spi_state`` >>
+rw [spi_tau_operations_def, rx_channel_enabled_op_def] >>
+fs [ref_rel_def, IS_STATE_REL_def],
+(* dr_rx_check_rxs and rx_channel_enabled *)
+DISJ1_TAC >>
+rw [local_tr_cases, spi_tr_cases, SPI_TAU_ENABLE_def] >>
+EXISTS_TAC ``dr:driver_state`` >>
+EXISTS_TAC ``spi_tau_operations spi:spi_state`` >>
+rw [spi_tau_operations_def, rx_channel_enabled_op_def] >>
+fs [ref_rel_def, IS_STATE_REL_def],
+(* dr_rx_conf_issued and rx_conf_ready *)
+DISJ2_TAC >>
+EXISTS_TAC ``SUC 0:num`` >>
+rw [n_tau_tr_def, local_tr_cases, driver_tr_cases, spi_tr_cases, 
+DR_WR_ENABLE_def, GSYM LEFT_EXISTS_AND_THM, DR_TAU_ENABLE_def, 
+SPI_TAU_ENABLE_def, DR_RD_ENABLE_def] >>
+EXISTS_TAC ``dr_write_state dr: driver_state`` >>
+EXISTS_TAC ``spi_tau_operations (write_SPI_regs (THE (dr_write_address dr)) (THE (dr_write_value dr)) spi)`` >>
+rw [] >|
+[DISJ2_TAC >> 
+DISJ1_TAC >>
+NTAC 4 DISJ2_TAC >>
+DISJ1_TAC >>
+rw [write_SPI_regs_def, dr_write_address_def, dr_write_value_def, dr_write_def, 
+dr_write_ch0ctrl_def, write_CH0CTRL_def , SPI0_CH0CTRL_def, SPI0_PA_RANGE_def, 
+SPI0_END_def, SPI0_START_def, SPI0_SYSCONFIG_def, SPI0_MODULCTRL_def, SPI0_CH0CONF_def],
+fs [write_SPI_regs_def, dr_write_address_def, dr_write_value_def, dr_write_state_def, 
+dr_write_def, dr_write_ch0ctrl_def, write_CH0CTRL_def] >>
+rw [SPI0_CH0CTRL_def, SPI0_PA_RANGE_def, SPI0_END_def, SPI0_START_def, SPI0_SYSCONFIG_def, 
+SPI0_MODULCTRL_def, SPI0_CH0CONF_def, spi_tau_operations_def, rx_channel_enabled_op_def] >>
+fs [ref_rel_def, IS_STATE_REL_def]],
+(* dr_rx_idle and spi_ready *)
+DISJ2_TAC >>
+EXISTS_TAC ``SUC 1:num`` >>
+rw [n_tau_tr_def, n_tau_tr_SUC, local_tr_cases, driver_tr_cases, spi_tr_cases,
+DR_WR_ENABLE_def, GSYM LEFT_EXISTS_AND_THM, GSYM RIGHT_EXISTS_AND_THM,
+DR_TAU_ENABLE_def, SPI_TAU_ENABLE_def, DR_RD_ENABLE_def] >>
+rw [dr_write_state_def, dr_write_def, dr_write_ch0conf_rx_def] >>
+`(write_SPI_regs (THE (dr_write_address dr)) (THE (dr_write_value dr)) spi) = 
+spi with <| state := rx_conf_ready; 
+regs := spi.regs with CH0CONF := spi.regs.CH0CONF with
+<|TRM := 1w; FORCE := 1w |> |>` by rw [write_SPI_regs_def, dr_write_address_def, 
+dr_write_value_def, dr_write_def, dr_write_ch0conf_rx_def, write_CH0CONF_comb_def, 
+write_CH0CONF_rx_def, SPI0_CH0CTRL_def, SPI0_PA_RANGE_def, SPI0_END_def, SPI0_START_def,
+SPI0_SYSCONFIG_def, SPI0_MODULCTRL_def, SPI0_CH0CONF_def] >>
+fs [dr_write_ch0ctrl_def] >>
+EXISTS_TAC ``dr with state := dr_rx_read_rxs`` >>
+EXISTS_TAC ``spi_tau_operations 
+(write_SPI_regs (THE (dr_write_address (dr with state := dr_rx_conf_issued)))
+(THE (dr_write_value (dr with state := dr_rx_conf_issued)))
+(spi with <| state := rx_conf_ready; regs := spi.regs with CH0CONF := spi.regs.CH0CONF with
+<|TRM := 1w; FORCE := 1w |> |>))`` >>
+rw [] >|
+[DISJ1_TAC >> 
+NTAC 4 DISJ2_TAC >> 
+DISJ1_TAC >>
+rw [write_SPI_regs_def, dr_write_address_def, dr_write_value_def, dr_write_def, 
+SPI0_CH0CTRL_def, SPI0_PA_RANGE_def, SPI0_END_def, SPI0_START_def, SPI0_SYSCONFIG_def, 
+SPI0_MODULCTRL_def, SPI0_CH0CONF_def, dr_write_ch0ctrl_def, write_CH0CTRL_def],
+rw [write_SPI_regs_def, dr_write_address_def, dr_write_value_def, dr_write_def, 
+SPI0_CH0CTRL_def, SPI0_PA_RANGE_def, SPI0_END_def, SPI0_START_def, SPI0_SYSCONFIG_def, 
+SPI0_MODULCTRL_def, SPI0_CH0CONF_def, dr_write_ch0ctrl_def] >>
+rw [write_CH0CTRL_def, spi_tau_operations_def, rx_channel_enabled_op_def] >>
+fs [ref_rel_def, IS_STATE_REL_def]]]);
+
+(* ref_rel holds if ds_abs1 performs tau_spi transition and ds_abs1.state = abs1_rx_update *)
+val ref_rel_holds_tau_spi_abs1_rx_update = store_thm("ref_rel_holds_tau_spi_abs1_rx_update",
+``!spi dr ds_abs1.
+(ref_rel ds_abs1 (dr,spi)) /\ (ds_abs1.state = abs1_rx_update) /\
+(IS_STATE_REL ds_abs1 dr spi) ==>
+?dr' spi'. (local_tr (dr, spi) tau (dr', spi')) /\ 
+(ref_rel (spi_abs1_rx_operations ds_abs1) (dr', spi'))``,
+rw [spi_abs1_rx_operations_def, spi_abs1_rx_update_op_def] >>
+`(dr.state = dr_rx_read_rxs /\ spi.state = rx_update_RX0) \/
+(dr.state = dr_rx_check_rxs /\ spi.state = rx_update_RX0)` by fs [IS_STATE_REL_def] >>
+rw [local_tr_cases, spi_tr_cases, SPI_TAU_ENABLE_def] >>
+EXISTS_TAC ``dr:driver_state`` >>
+EXISTS_TAC ``spi_tau_operations spi:spi_state`` >>
+rw [spi_tau_operations_def, rx_update_RX0_op_def] >>
+fs [ref_rel_def, IS_STATE_REL_def] >>
+SIMP_TAC (std_ss ++ WORD_BIT_EQ_ss) []);
+
+(* ref_rel holds if ds_abs1 performs tau_spi transition and ds_abs1.state = abs1_rx_next *)
+val ref_rel_holds_tau_spi_abs1_rx_next = store_thm("ref_rel_holds_tau_spi_abs1_rx_next",
+``!spi dr ds_abs1.
+(ref_rel ds_abs1 (dr,spi)) /\ (ds_abs1.state = abs1_rx_next) /\
+(IS_STATE_REL ds_abs1 dr spi) ==>
+?dr' spi'. (local_tr (dr, spi) tau (dr', spi')) /\ 
+(ref_rel (spi_abs1_rx_operations ds_abs1) (dr', spi'))``,
+rw [spi_abs1_rx_operations_def, spi_abs1_rx_next_op_def] >>
+`dr.state = dr_rx_fetch_data /\ spi.state = rx_update_RX0` by fs [IS_STATE_REL_def] >>
+rw [local_tr_cases, spi_tr_cases, SPI_TAU_ENABLE_def] >>
+EXISTS_TAC ``dr:driver_state`` >>
+EXISTS_TAC ``spi_tau_operations spi:spi_state`` >>
+rw [spi_tau_operations_def, rx_update_RX0_op_def] >>
+fs [ref_rel_def, IS_STATE_REL_def] >>
+SIMP_TAC (std_ss ++ WORD_BIT_EQ_ss) []);
+
+(* (dr',spi') exists for rx automaton *)
+val abs1_comb_hold_ref_rel_tau_spi_rx = store_thm("abs1_comb_hold_ref_rel_tau_spi_rx",
+``!spi dr ds_abs1.
+(ref_rel ds_abs1 (dr, spi)) /\ (SPI_ABS1_RX_ENABLE ds_abs1) ==>
+(?dr' spi'. (local_tr (dr, spi) tau (dr', spi')) /\ 
+(ref_rel (spi_abs1_rx_operations ds_abs1) (dr', spi'))) \/
+(?n dr' spi'. (n_tau_tr n local_tr (dr,spi) tau (dr',spi')) /\ 
+(ref_rel (spi_abs1_rx_operations ds_abs1) (dr',spi')))``,
+rw [SPI_ABS1_RX_ENABLE_def] >>
+`IS_STATE_REL ds_abs1 dr spi` by fs [ref_rel_def] >>
+rw [ref_rel_holds_tau_spi_abs1_rx_idle, ref_rel_holds_tau_spi_abs1_rx_update,
+ref_rel_holds_tau_spi_abs1_rx_next]);
+
+
+(* theorems related to xfer automaton *)
+(* ref_rel holds if ds_abs1 performs tau_spi transition and ds_abs1.state = abs1_xfer_idle *)
+val ref_rel_holds_tau_spi_abs1_xfer_idle = store_thm("ref_rel_holds_tau_spi_abs1_xfer_idle",
+``!spi dr ds_abs1.
+(ref_rel ds_abs1 (dr,spi)) /\ (ds_abs1.state = abs1_xfer_idle) /\
+(IS_STATE_REL ds_abs1 dr spi) ==>
+(?dr' spi'. (local_tr (dr, spi) tau (dr', spi')) /\ 
+(ref_rel (spi_abs1_xfer_operations ds_abs1) (dr', spi'))) \/
+(?n dr' spi'. n_tau_tr n local_tr (dr,spi) tau (dr',spi') /\
+ref_rel (spi_abs1_xfer_operations ds_abs1) (dr',spi'))``,
+rw [spi_abs1_xfer_operations_def, spi_abs1_xfer_idle_op_def] >>
+`(dr.state = dr_xfer_read_txs /\ spi.state = xfer_channel_enabled) \/
+(dr.state = dr_xfer_check_txs /\ spi.state = xfer_channel_enabled) \/
+(dr.state = dr_xfer_conf_issued /\ spi.state = xfer_conf_ready) \/
+(dr.state = dr_xfer_idle /\ spi.state = spi_ready)` by fs [IS_STATE_REL_def] >|
+[(* dr_xfer_read_txs and xfer_channel_enabled *)
+DISJ1_TAC >>
+rw [local_tr_cases, spi_tr_cases, SPI_TAU_ENABLE_def] >>
+Q.EXISTS_TAC `dr:driver_state` >>
+Q.EXISTS_TAC `spi_tau_operations spi` >>
+rw [spi_tau_operations_def, xfer_channel_enabled_op_def] >>
+fs [ref_rel_def, IS_STATE_REL_def],
+(* dr_xfer_check_txs and xfer_channel_enabled *)
+DISJ1_TAC >>
+rw [local_tr_cases, spi_tr_cases, SPI_TAU_ENABLE_def] >>
+Q.EXISTS_TAC `dr:driver_state` >>
+Q.EXISTS_TAC `spi_tau_operations spi` >>
+rw [spi_tau_operations_def, xfer_channel_enabled_op_def] >>
+fs [ref_rel_def, IS_STATE_REL_def],
+(* dr_xfer_conf_issued and xfer_conf_ready *)
+DISJ2_TAC >>
+EXISTS_TAC ``SUC 0:num`` >>
+rw [n_tau_tr_def, local_tr_cases, driver_tr_cases, spi_tr_cases, 
+DR_WR_ENABLE_def, GSYM LEFT_EXISTS_AND_THM, DR_TAU_ENABLE_def, 
+SPI_TAU_ENABLE_def, DR_RD_ENABLE_def] >>
+Q.EXISTS_TAC `dr_write_state dr` >>
+Q.EXISTS_TAC `spi_tau_operations (write_SPI_regs (THE (dr_write_address dr)) (THE (dr_write_value dr)) spi)` >>
+rw [] >|
+[DISJ2_TAC >>
+DISJ1_TAC >>
+NTAC 6 DISJ2_TAC >>
+DISJ1_TAC >>
+rw [write_SPI_regs_def, dr_write_address_def, dr_write_value_def, dr_write_def, 
+dr_write_ch0ctrl_def, write_CH0CTRL_def , SPI0_CH0CTRL_def, SPI0_PA_RANGE_def, 
+SPI0_END_def, SPI0_START_def, SPI0_SYSCONFIG_def, SPI0_MODULCTRL_def, SPI0_CH0CONF_def],
+fs [write_SPI_regs_def, dr_write_address_def, dr_write_value_def, dr_write_state_def, 
+dr_write_def, dr_write_ch0ctrl_def, write_CH0CTRL_def] >>
+rw [SPI0_CH0CTRL_def, SPI0_PA_RANGE_def, SPI0_END_def, SPI0_START_def, SPI0_SYSCONFIG_def, 
+SPI0_MODULCTRL_def, SPI0_CH0CONF_def, spi_tau_operations_def, xfer_channel_enabled_op_def] >>
+fs [ref_rel_def, IS_STATE_REL_def]],
+(* dr_xfer_idle and spi_ready *)
+DISJ2_TAC >>
+EXISTS_TAC ``SUC 1:num`` >>
+rw [n_tau_tr_def, n_tau_tr_SUC, local_tr_cases, driver_tr_cases, spi_tr_cases,
+DR_WR_ENABLE_def, GSYM LEFT_EXISTS_AND_THM, GSYM RIGHT_EXISTS_AND_THM,
+DR_TAU_ENABLE_def, SPI_TAU_ENABLE_def, DR_RD_ENABLE_def] >>
+rw [dr_write_state_def, dr_write_def, dr_write_ch0conf_xfer_def] >>
+`(write_SPI_regs (THE (dr_write_address dr)) (THE (dr_write_value dr)) spi) = 
+spi with <| state := xfer_conf_ready; 
+regs := spi.regs with CH0CONF := spi.regs.CH0CONF with
+<|TRM := 0w; FORCE := 1w |> |>` by rw [write_SPI_regs_def, dr_write_address_def, 
+dr_write_value_def, dr_write_def, dr_write_ch0conf_xfer_def, write_CH0CONF_comb_def, 
+write_CH0CONF_xfer_def, SPI0_CH0CTRL_def, SPI0_PA_RANGE_def, SPI0_END_def, SPI0_START_def,
+SPI0_SYSCONFIG_def, SPI0_MODULCTRL_def, SPI0_CH0CONF_def] >>
+fs [dr_write_ch0ctrl_def] >>
+Q.EXISTS_TAC `dr with state := dr_xfer_read_txs` >>
+Q.EXISTS_TAC `spi_tau_operations 
+(write_SPI_regs (THE (dr_write_address (dr with state := dr_xfer_conf_issued)))
+(THE (dr_write_value (dr with state := dr_xfer_conf_issued)))
+(spi with <| state := xfer_conf_ready; regs := spi.regs with CH0CONF := spi.regs.CH0CONF with
+<|TRM := 0w; FORCE := 1w |> |>))` >>
+rw [] >|
+[DISJ1_TAC >> 
+NTAC 6 DISJ2_TAC >> 
+DISJ1_TAC >>
+rw [write_SPI_regs_def, dr_write_address_def, dr_write_value_def, dr_write_def, 
+SPI0_CH0CTRL_def, SPI0_PA_RANGE_def, SPI0_END_def, SPI0_START_def, SPI0_SYSCONFIG_def, 
+SPI0_MODULCTRL_def, SPI0_CH0CONF_def, dr_write_ch0ctrl_def, write_CH0CTRL_def],
+rw [write_SPI_regs_def, dr_write_address_def, dr_write_value_def, dr_write_def, 
+SPI0_CH0CTRL_def, SPI0_PA_RANGE_def, SPI0_END_def, SPI0_START_def, SPI0_SYSCONFIG_def, 
+SPI0_MODULCTRL_def, SPI0_CH0CONF_def, dr_write_ch0ctrl_def] >>
+rw [write_CH0CTRL_def, spi_tau_operations_def, xfer_channel_enabled_op_def] >>
+fs [ref_rel_def, IS_STATE_REL_def]]]);
+
+(* ref_rel holds if ds_abs1 performs tau_spi transition and ds_abs1.state = abs1_xfer_data *)
+val ref_rel_holds_tau_spi_abs1_xfer_data = store_thm("ref_rel_holds_tau_spi_abs1_xfer_data",
+``!spi dr ds_abs1.
+(ref_rel ds_abs1 (dr,spi)) /\ (ds_abs1.state = abs1_xfer_data) /\
+(IS_STATE_REL ds_abs1 dr spi) ==>
+?dr' spi'. (local_tr (dr, spi) tau (dr', spi')) /\ 
+(ref_rel (spi_abs1_xfer_operations ds_abs1) (dr', spi'))``,
+rw [spi_abs1_xfer_operations_def, spi_abs1_xfer_data_op_def] >>
+`(dr.state = dr_xfer_read_rxs /\ spi.state = xfer_trans_data) \/
+(dr.state = dr_xfer_check_rxs /\ spi.state = xfer_trans_data)` by fs [IS_STATE_REL_def] >>
+rw [local_tr_cases, spi_tr_cases, SPI_TAU_ENABLE_def] >>
+EXISTS_TAC ``dr:driver_state`` >>
+EXISTS_TAC ``spi_tau_operations spi:spi_state`` >>
+rw [spi_tau_operations_def, xfer_trans_data_op_def] >>
+fs [ref_rel_def, IS_STATE_REL_def]);
+
+(* ref_rel holds if ds_abs1 performs tau_spi transition and ds_abs1.state = abs1_xfer_update *)
+val ref_rel_holds_tau_spi_abs1_xfer_update = store_thm("ref_rel_holds_tau_spi_abs1_xfer_update",
+``!spi dr ds_abs1.
+(ref_rel ds_abs1 (dr,spi)) /\ (ds_abs1.state = abs1_xfer_update) /\
+(IS_STATE_REL ds_abs1 dr spi) ==>
+?dr' spi'. (local_tr (dr, spi) tau (dr', spi')) /\ 
+(ref_rel (spi_abs1_xfer_operations ds_abs1) (dr', spi'))``,
+rw [spi_abs1_xfer_operations_def, spi_abs1_xfer_update_op_def] >>
+`(dr.state = dr_xfer_read_rxs /\ spi.state = xfer_update_RX0) \/
+(dr.state = dr_xfer_check_rxs /\ spi.state = xfer_update_RX0)` by fs [IS_STATE_REL_def] >>
+rw [local_tr_cases, spi_tr_cases, SPI_TAU_ENABLE_def] >>
+EXISTS_TAC ``dr:driver_state`` >>
+EXISTS_TAC ``spi_tau_operations spi:spi_state`` >>
+rw [spi_tau_operations_def, xfer_update_RX0_op_def] >>
+fs [ref_rel_def, IS_STATE_REL_def] >>
+SIMP_TAC (std_ss++WORD_BIT_EQ_ss) []);
+
+(* (dr',spi') exists for xfer automaton *)
+val abs1_comb_hold_ref_rel_tau_spi_xfer = store_thm("abs1_comb_hold_ref_rel_tau_spi_xfer",
+``!spi dr ds_abs1.
+(ref_rel ds_abs1 (dr, spi)) /\ (SPI_ABS1_XFER_ENABLE ds_abs1) ==>
+(?dr' spi'. (local_tr (dr, spi) tau (dr', spi')) /\ 
+(ref_rel (spi_abs1_xfer_operations ds_abs1) (dr', spi'))) \/
+(?n dr' spi'. (n_tau_tr n local_tr (dr,spi) tau (dr',spi')) /\ 
+(ref_rel (spi_abs1_xfer_operations ds_abs1) (dr',spi')))``,
+rw [SPI_ABS1_XFER_ENABLE_def] >>
+`IS_STATE_REL ds_abs1 dr spi` by fs [ref_rel_def] >>
+rw [ref_rel_holds_tau_spi_abs1_xfer_idle, ref_rel_holds_tau_spi_abs1_xfer_data,
+ref_rel_holds_tau_spi_abs1_xfer_update]);
+
+(* simulation: (dr',spi') exists and holds the ref_rel when ds_abs1 has tau_spi *)
+val abs1_comb_hold_ref_rel_tau_spi = store_thm("abs1_comb_hold_ref_rel_tau_spi",
+``!spi dr ds_abs1 ds_abs1'.
+(ref_rel ds_abs1 (dr, spi)) /\ (ds_abs1_spi_tr ds_abs1 tau_spi ds_abs1') ==>
+(?dr' spi'. (local_tr (dr, spi) tau (dr', spi')) /\ (ref_rel ds_abs1' (dr', spi'))) \/
+(?n dr' spi'. (n_tau_tr n local_tr (dr,spi) tau (dr',spi')) /\ (ref_rel ds_abs1' (dr',spi')))``,
+rw [ds_abs1_spi_tr_cases] >>
+rw [abs1_comb_hold_ref_rel_tau_spi_tx, abs1_comb_hold_ref_rel_tau_spi_rx,
+abs1_comb_hold_ref_rel_tau_spi_xfer]);
+
+val _ = export_theory();
