abs1_comb_thm/abs1_comb_weak_bisimulationScript.sml
@@ -1,0 +1,91 @@
+open HolKernel bossLib boolLib Parse;
+open SPI_stateTheory SPI_relationTheory weak_bisimulationTheory;
+open driver_stateTheory driver_relationTheory;
+open ds_abs1_stateTheory ref_relTheory ds_abs1_relTheory;
+open ref_rel_holds_call_lblTheory ref_rel_holds_trans_lblTheory;
+open comb_abs1_hold_ref_rel_spi_trTheory comb_abs1_hold_ref_rel_dr_trTheory comb_abs1_hold_ref_rel_RD_RETheory comb_abs1_hold_ref_rel_WR_UPTheory;
+open abs1_comb_hold_ref_rel_tau_spiTheory abs1_comb_hold_ref_rel_tau_drTheory abs1_comb_hold_ref_rel_tau_combTheory;
+
+val _ = new_theory "abs1_comb_weak_bisimulation";
+
+(* weak simulation if (dr,spi) -> (dr', spi') *)
+(* simulation: ds_abs1' exists when lbl is not tau *)
+val comb_abs1_weak_simulation_lbl_not_tau = store_thm("comb_abs1_weak_simulation_lbl_not_tau",
+``!spi dr ds_abs1 lbl dr' spi'.
+(ref_rel ds_abs1 (dr, spi)) /\ (local_tr (dr, spi) lbl (dr', spi')) ==>
+(lbl <> tau ==> 
+?ds_abs1'. (ds_abs1_tr ds_abs1 lbl ds_abs1') /\ (ref_rel ds_abs1' (dr', spi')))``,
+rw [local_tr_cases] >>
+METIS_TAC [comb_abs1_hold_ref_rel_call_init, comb_abs1_hold_ref_rel_call_tx,
+comb_abs1_hold_ref_rel_call_rx, comb_abs1_hold_ref_rel_call_xfer, 
+comb_abs1_hold_ref_rel_TX, comb_abs1_hold_ref_rel_RX,
+comb_abs1_hold_ref_rel_XFER]);
+
+(* simulation: ds_abs1 or ds_abs1' exists for ref_rel holding when lbl is tau *)
+val comb_abs1_weak_simulation_tau = store_thm("comb_abs1_weak_simulation_tau",
+``!spi dr ds_abs1 dr' spi'.
+(ref_rel ds_abs1 (dr, spi)) /\ (local_tr (dr, spi) tau (dr', spi')) ==>
+(ref_rel ds_abs1 (dr', spi')) \/ 
+(?ds_abs1'. (ds_abs1_tr ds_abs1 tau ds_abs1') /\ (ref_rel ds_abs1' (dr', spi')))``,
+rw [local_tr_cases] >> 
+METIS_TAC [comb_abs1_hold_ref_rel_driver_tr, comb_abs1_hold_ref_rel_spi_tr,
+comb_abs1_hold_ref_rel_WR_UP, comb_abs1_hold_ref_rel_RD_RE]);
+
+(* simulation: when (dr, spi) performs state transition, ds_abs1 is simulated to (dr,spi). *)
+val comb_abs1_weak_simulation = store_thm("comb_abs1_weak_simulation",
+``!spi dr ds_abs1 lbl dr' spi'.
+(ref_rel ds_abs1 (dr,spi)) /\ (local_tr (dr,spi) lbl (dr',spi')) ==>
+(lbl = tau ==>
+(?ds_abs1'. (ds_abs1_tr ds_abs1 lbl ds_abs1') /\ (ref_rel ds_abs1' (dr',spi'))) \/
+(ref_rel ds_abs1 (dr',spi'))) /\
+(lbl <> tau ==>
+?ds_abs1'. (ds_abs1_tr ds_abs1 lbl ds_abs1') /\ (ref_rel ds_abs1' (dr',spi')))``,
+rw []  >>
+METIS_TAC [comb_abs1_weak_simulation_tau, comb_abs1_weak_simulation_lbl_not_tau]);
+
+(* weak simulation if ds_abs1 -> ds_abs1' *)
+(* simulation: (dr', spi') exists when lbl is not tau *)
+val abs1_comb_weak_simulation_lbl_not_tau = store_thm("abs1_comb_weak_simulation_lbl_not_tau",
+``!spi dr ds_abs1 lbl ds_abs1'.
+(ref_rel ds_abs1 (dr, spi)) /\ (ds_abs1_tr ds_abs1 lbl ds_abs1') ==>
+(lbl <> tau ==> ?dr' spi'. (local_tr (dr, spi) lbl (dr', spi')) /\ 
+(ref_rel ds_abs1' (dr', spi')))``,
+rw [ds_abs1_tr_cases] >>
+rw [abs1_comb_hold_ref_rel_TX, abs1_comb_hold_ref_rel_RX, abs1_comb_hold_ref_rel_XFER] >>
+METIS_TAC [ds_abs1_tr_cases, abs1_comb_hold_ref_rel_call_init, 
+abs1_comb_hold_ref_rel_call_init, ds_abs1_tr_cases, abs1_comb_hold_ref_rel_call_tx,
+abs1_comb_hold_ref_rel_call_rx, abs1_comb_hold_ref_rel_call_xfer]);
+
+(* simulation: (dr',spi') exists when lbl is tau *)
+val abs1_comb_weak_simulation_tau = store_thm("abs1_comb_weak_simulation_tau",
+``!spi dr ds_abs1 ds_abs1'.
+(ref_rel ds_abs1 (dr, spi)) /\ (ds_abs1_tr ds_abs1 tau ds_abs1') ==>
+(?dr' spi'. (local_tr (dr,spi) tau (dr', spi')) /\ (ref_rel ds_abs1' (dr', spi'))) \/
+(?n dr' spi'. (n_tau_tr n local_tr (dr, spi) tau (dr', spi')) /\
+(ref_rel ds_abs1' (dr', spi')))``,
+rw [ds_abs1_tr_cases] >>
+METIS_TAC [abs1_comb_hold_ref_rel_tau_spi, abs1_comb_hold_ref_rel_tau_dr,
+abs1_comb_hold_ref_rel_tau_comb]);
+
+(* simulation: when ds_abs1 performs state transition, (dr,spi) is simulated to ds_abs1 *)
+val abs1_comb_weak_simulation = store_thm("abs1_comb_weak_simulation",
+``!spi dr ds_abs1 lbl ds_abs1'.
+(ref_rel ds_abs1 (dr,spi)) /\ (ds_abs1_tr ds_abs1 lbl ds_abs1') ==>
+(?dr' spi'. (local_tr (dr, spi) lbl (dr', spi')) /\ (ref_rel ds_abs1' (dr',spi'))) \/
+(?n dr' spi'. (n_tau_tr n local_tr (dr,spi) lbl (dr',spi')) /\ (ref_rel ds_abs1' (dr',spi')))``,
+rw [] >>
+Cases_on `lbl = tau` >>
+METIS_TAC [abs1_comb_weak_simulation_tau, abs1_comb_weak_simulation_lbl_not_tau]);
+
+(* ref_rel is the weak bisimulation relation for ds_abs1 and (dr,spi) 
+   state transition systems *)
+val weak_bisimulation_abs1_comb = store_thm("weak_bisimulation_abs1_comb",
+``weak_bisim ref_rel ds_abs1_tr local_tr``,
+rw [weak_bisim_def, weak_tr_def] >>
+Cases_on `s2` >|
+[METIS_TAC [abs1_comb_weak_simulation],
+Cases_on `s2'` >>
+METIS_TAC [comb_abs1_weak_simulation]]);
+
+
+val _ = export_theory();
