abs1_comb_thm/ref_rel_holds_call_lblScript.sml
@@ -10,7 +10,7 @@ val _ = new_theory "ref_rel_holds_call_lbl";
 (* If dr.state = dr_init_pre, then abs1.state = init_pre according to ref_rel *)
 val dr_init_pre_imply_abs1_init_pre = store_thm("dr_init_pre_imply_abs1_init_pre",
 ``!(spi:spi_state) (dr:driver_state) (ds_abs1:ds_abs1_state).
-(ref_rel ds_abs1 dr spi) /\ (dr.state = dr_init_pre) ==>
+(ref_rel ds_abs1 (dr, spi)) /\ (dr.state = dr_init_pre) ==>
 ds_abs1.state = abs1_init_pre``,
 rw [] >>
 `IS_STATE_REL ds_abs1 dr spi` by METIS_TAC[ref_rel_def] >>
@@ -56,7 +56,7 @@ rw []);
 (* If dr.state = dr_ready, then abs1.state = abs1_ready according to ref_rel *)
 val dr_ready_imply_abs1_ready = store_thm("dr_ready_imply_abs1_ready",
 ``!(spi:spi_state) (dr:driver_state) (ds_abs1:ds_abs1_state).
-(ref_rel ds_abs1 dr spi) /\ (dr.state = dr_ready) ==>
+(ref_rel ds_abs1 (dr,spi)) /\ (dr.state = dr_ready) ==>
 ds_abs1.state = abs1_ready``,
 rw [] >>
 `IS_STATE_REL ds_abs1 dr spi` by METIS_TAC[ref_rel_def] >>
@@ -99,11 +99,11 @@ rw [] >>
 Cases_on `ds_abs1.state` >>
 rw []);
 
-(* bisimulation: ds_abs1' exits for call_init label *)
-val abs1_comb_hold_ref_rel_call_init = store_thm("abs1_comb_hold_ref_rel_call_init",
+(* ds_abs1' exits for call_init label *)
+val comb_abs1_hold_ref_rel_call_init = store_thm("comb_abs1_hold_ref_rel_call_init",
 ``!(spi:spi_state) (dr:driver_state) (ds_abs1:ds_abs1_state) (dr':driver_state).
-(ref_rel ds_abs1 dr spi) /\ (driver_tr dr call_init dr') ==>
-?ds_abs1'. (ds_abs1_tr ds_abs1 call_init ds_abs1') /\ (ref_rel ds_abs1' dr' spi)``,
+(ref_rel ds_abs1 (dr, spi)) /\ (driver_tr dr call_init dr') ==>
+?ds_abs1'. (ds_abs1_tr ds_abs1 call_init ds_abs1') /\ (ref_rel ds_abs1' (dr', spi))``,
 rw [driver_tr_cases, ds_abs1_tr_cases] >|
 [ (* abs1_init_pre *)
 METIS_TAC [dr_init_pre_imply_abs1_init_pre],
@@ -120,12 +120,12 @@ rw [call_init_ds_abs1_def, call_init_dr_def] >>
 FULL_SIMP_TAC std_ss [ref_rel_def, IS_STATE_REL_def] >>
 rw []]);
 
-(* bisimulation: (dr',spi') exists for call_init label *)
-val comb_abs1_hold_ref_rel_call_init = store_thm("comb_abs1_hold_ref_rel_call_init",
+(* (dr',spi') exists for call_init label *)
+val abs1_comb_hold_ref_rel_call_init = store_thm("abs1_comb_hold_ref_rel_call_init",
 ``!(spi:spi_state) (dr:driver_state) (ds_abs1:ds_abs1_state) (ds_abs1':ds_abs1_state).
-(ref_rel ds_abs1 dr spi) /\ (ds_abs1_tr ds_abs1 call_init ds_abs1') ==>
+(ref_rel ds_abs1 (dr, spi)) /\ (ds_abs1_tr ds_abs1 call_init ds_abs1') ==>
 ?dr' spi'. (local_tr (dr, spi) call_init (dr', spi')) /\
-(ref_rel ds_abs1' dr' spi')``,
+(ref_rel ds_abs1' (dr', spi'))``,
 rw [ds_abs1_tr_cases, local_tr_cases, driver_tr_cases] >|
 [FULL_SIMP_TAC std_ss [ref_rel_def, IS_STATE_REL_def],
 rw [call_init_ds_abs1_def, call_init_dr_def] >>
@@ -136,11 +136,11 @@ rw [call_init_ds_abs1_def, call_init_dr_def] >>
 FULL_SIMP_TAC std_ss [ref_rel_def, IS_STATE_REL_def] >>
 rw []]);
 
-(* bisimulation: ds_abs1' exists for call_tx label *)
-val abs1_comb_hold_ref_rel_call_tx = store_thm("abs1_comb_hold_ref_rel_call_tx",
+(* ds_abs1' exists for call_tx label *)
+val comb_abs1_hold_ref_rel_call_tx = store_thm("comb_abs1_hold_ref_rel_call_tx",
 ``!(spi:spi_state) (dr:driver_state) (ds_abs1:ds_abs1_state) (buffer:word8 list) (dr':driver_state).
-(ref_rel ds_abs1 dr spi) /\ (driver_tr dr (call_tx buffer) dr') ==>
-?ds_abs1'. (ds_abs1_tr ds_abs1 (call_tx buffer) ds_abs1') /\ (ref_rel ds_abs1' dr' spi)``,
+(ref_rel ds_abs1 (dr, spi)) /\ (driver_tr dr (call_tx buffer) dr') ==>
+?ds_abs1'. (ds_abs1_tr ds_abs1 (call_tx buffer) ds_abs1') /\ (ref_rel ds_abs1' (dr', spi))``,
 rw [driver_tr_cases, ds_abs1_tr_cases] >|
 [(* check the state *)
 METIS_TAC [dr_ready_imply_abs1_ready],
@@ -150,12 +150,12 @@ rw [call_tx_ds_abs1_def, call_tx_dr_def] >>
 FULL_SIMP_TAC std_ss [ref_rel_def, IS_STATE_REL_def] >>
 rw []]);
 
-(* bisimulation: (dr',spi') exists for call_tx label *)
-val comb_abs1_hold_ref_rel_call_tx = store_thm("comb_abs1_hold_ref_rel_call_tx",
+(* (dr',spi') exists for call_tx label *)
+val abs1_comb_hold_ref_rel_call_tx = store_thm("abs1_comb_hold_ref_rel_call_tx",
 ``!(spi:spi_state) (dr:driver_state) (ds_abs1:ds_abs1_state) (buffer:word8 list) (ds_abs1':ds_abs1_state).
-(ref_rel ds_abs1 dr spi) /\ (ds_abs1_tr ds_abs1 (call_tx buffer) ds_abs1') ==>
+(ref_rel ds_abs1 (dr, spi)) /\ (ds_abs1_tr ds_abs1 (call_tx buffer) ds_abs1') ==>
 ?dr' spi'. (local_tr (dr, spi) (call_tx buffer) (dr', spi')) /\
-(ref_rel ds_abs1' dr' spi')``,
+(ref_rel ds_abs1' (dr', spi'))``,
 rw [ds_abs1_tr_cases, local_tr_cases, driver_tr_cases] >|
 [FULL_SIMP_TAC std_ss [ref_rel_def, IS_STATE_REL_def],
 rw [call_tx_ds_abs1_def, call_tx_dr_def] >>
@@ -163,10 +163,10 @@ FULL_SIMP_TAC std_ss [ref_rel_def, IS_STATE_REL_def] >>
 rw []]);
 
 (* bisimulation: ds_abs1' exists for call_rx label *)
-val abs1_comb_hold_ref_rel_call_rx = store_thm("abs1_comb_hold_ref_rel_call_rx",
+val comb_abs1_hold_ref_rel_call_rx = store_thm("comb_abs1_hold_ref_rel_call_rx",
 ``!(spi:spi_state) (dr:driver_state) (ds_abs1:ds_abs1_state) (length: num) (dr':driver_state).
-(ref_rel ds_abs1 dr spi) /\ (driver_tr dr (call_rx length) dr') ==>
-?ds_abs1'. (ds_abs1_tr ds_abs1 (call_rx length) ds_abs1') /\ (ref_rel ds_abs1' dr' spi)``,
+(ref_rel ds_abs1 (dr, spi)) /\ (driver_tr dr (call_rx length) dr') ==>
+?ds_abs1'. (ds_abs1_tr ds_abs1 (call_rx length) ds_abs1') /\ (ref_rel ds_abs1' (dr', spi))``,
 rw [driver_tr_cases, ds_abs1_tr_cases] >|
 [(* check the state *)
 METIS_TAC [dr_ready_imply_abs1_ready],
@@ -177,11 +177,11 @@ FULL_SIMP_TAC std_ss [ref_rel_def, IS_STATE_REL_def] >>
 rw []]);
 
 (* bisimulation: (ds',spi') exists for call_rx label *)
-val comb_abs1_hold_ref_rel_call_rx = store_thm("comb_abs1_hold_ref_rel_call_rx",
+val abs1_comb_hold_ref_rel_call_rx = store_thm("abs1_comb_hold_ref_rel_call_rx",
 ``!(spi:spi_state) (dr:driver_state) (ds_abs1:ds_abs1_state) (length: num) (dr':driver_state) (ds_abs1':ds_abs1_state).
-(ref_rel ds_abs1 dr spi) /\ (ds_abs1_tr ds_abs1 (call_rx length) ds_abs1') ==>
+(ref_rel ds_abs1 (dr, spi)) /\ (ds_abs1_tr ds_abs1 (call_rx length) ds_abs1') ==>
 ?dr' spi'. (local_tr (dr, spi) (call_rx length) (dr', spi')) /\ 
-(ref_rel ds_abs1' dr' spi')``,
+(ref_rel ds_abs1' (dr', spi'))``,
 rw [ds_abs1_tr_cases, local_tr_cases, driver_tr_cases] >|
 [FULL_SIMP_TAC std_ss [ref_rel_def, IS_STATE_REL_def],
 rw [call_rx_ds_abs1_def, call_rx_dr_def] >>
@@ -189,10 +189,11 @@ FULL_SIMP_TAC std_ss [ref_rel_def, IS_STATE_REL_def] >>
 rw []]); 
 
 (* bisimulation: ds_abs1' exists for call_xfer label *)
-val abs1_comb_hold_ref_rel_call_xfer = store_thm("abs1_comb_hold_ref_rel_call_xfer",
+val comb_abs1_hold_ref_rel_call_xfer = store_thm("comb_abs1_hold_ref_rel_call_xfer",
 ``!(spi:spi_state) (dr:driver_state) (ds_abs1:ds_abs1_state) (buffer:word8 list) (dr':driver_state) (ds_abs1':ds_abs1_state).
-(ref_rel ds_abs1 dr spi) /\ (driver_tr dr (call_xfer buffer) dr') ==>
-?ds_abs1'. (ds_abs1_tr ds_abs1 (call_xfer buffer) ds_abs1') /\ (ref_rel ds_abs1' dr' spi)``,
+(ref_rel ds_abs1 (dr, spi)) /\ (driver_tr dr (call_xfer buffer) dr') ==>
+?ds_abs1'. (ds_abs1_tr ds_abs1 (call_xfer buffer) ds_abs1') /\ 
+(ref_rel ds_abs1' (dr', spi))``,
 rw [driver_tr_cases, ds_abs1_tr_cases] >|
 [(* check the state *)
 METIS_TAC [dr_ready_imply_abs1_ready],
@@ -203,11 +204,11 @@ FULL_SIMP_TAC std_ss [ref_rel_def, IS_STATE_REL_def] >>
 rw []]);
 
 (* bisimulation: (dr',spi') exists for call_xfer label *)
-val comb_abs1_hold_ref_rel_call_xfer = store_thm("comb_abs1_hold_ref_rel_call_xfer",
+val abs1_comb_hold_ref_rel_call_xfer = store_thm("abs1_comb_hold_ref_rel_call_xfer",
 ``!(spi:spi_state) (dr:driver_state) (ds_abs1:ds_abs1_state) (buffer:word8 list) (ds_abs1':ds_abs1_state).
-(ref_rel ds_abs1 dr spi) /\ (ds_abs1_tr ds_abs1 (call_xfer buffer) ds_abs1') ==>
+(ref_rel ds_abs1 (dr, spi)) /\ (ds_abs1_tr ds_abs1 (call_xfer buffer) ds_abs1') ==>
 ?dr' spi'. (local_tr (dr, spi) (call_xfer buffer) (dr', spi')) /\
-(ref_rel ds_abs1' dr' spi')``,
+(ref_rel ds_abs1' (dr', spi'))``,
 rw [ds_abs1_tr_cases, local_tr_cases, driver_tr_cases] >|
 [FULL_SIMP_TAC std_ss [ref_rel_def, IS_STATE_REL_def],
 rw [call_xfer_ds_abs1_def, call_xfer_dr_def] >>
