abs1_comb_thm/ref_rel_holds_trans_lblScript.sml
@@ -11,7 +11,7 @@ val _ = new_theory "ref_rel_holds_trans_lbl";
 (* If spi.state = tx_trans_done or tx_trans_next, then ds_abs1 is also able to perform TX label transition *)
 val spi_tx_trans_done_imply_abs1_tx_enable = store_thm("spi_tx_trans_done_imply_abs1_tx_enable",
 ``!(spi:spi_state) (dr:driver_state) (ds_abs1:ds_abs1_state).
-(ref_rel ds_abs1 dr spi) /\ 
+(ref_rel ds_abs1 (dr, spi)) /\ 
 (spi.state = tx_trans_done \/ spi.state = tx_trans_next) ==>
 (ABS1_TX_LBL_ENABLE ds_abs1)``,
 rw [ABS1_TX_LBL_ENABLE_def] >>
@@ -25,10 +25,10 @@ Cases_on `spi.state` >>
 rw []);
 
 (* bisimulation: ds_abs1' exists for TX label *)
-val abs1_comb_hold_ref_rel_TX = store_thm("abs1_comb_hold_ref_rel_TX",
+val comb_abs1_hold_ref_rel_TX = store_thm("comb_abs1_hold_ref_rel_TX",
 ``!(spi:spi_state) (dr:driver_state) (ds_abs1:ds_abs1_state) (data:word8 option) (spi':spi_state).
-(ref_rel ds_abs1 dr spi) /\ (spi_tr spi (TX data) spi') ==>
-?ds_abs1'. (ds_abs1_tr ds_abs1 (TX data) ds_abs1') /\ (ref_rel ds_abs1' dr spi')``,
+(ref_rel ds_abs1 (dr, spi)) /\ (spi_tr spi (TX data) spi') ==>
+?ds_abs1'. (ds_abs1_tr ds_abs1 (TX data) ds_abs1') /\ (ref_rel ds_abs1' (dr, spi'))``,
 rw [spi_tr_cases] >>
 `ABS1_TX_LBL_ENABLE ds_abs1` by METIS_TAC[spi_tx_trans_done_imply_abs1_tx_enable] >>
 rw [ds_abs1_tr_cases] >|
@@ -53,12 +53,12 @@ tx_TX_op_state_def, tx_TX_op_def, tx_trans_next_op_def] >>
 FULL_SIMP_TAC std_ss [ref_rel_def, IS_STATE_REL_def] >>
 rw []]);
 
-(* bisimulation: (dr',spi') exists for TX label *)
-val comb_abs1_hold_ref_rel_TX = store_thm("comb_abs1_hold_ref_rel_TX",
+(* (dr',spi') exists for TX label *)
+val abs1_comb_hold_ref_rel_TX = store_thm("abs1_comb_hold_ref_rel_TX",
 ``!(spi:spi_state) (dr:driver_state) (ds_abs1:ds_abs1_state).
-(ref_rel ds_abs1 dr spi) /\ (ABS1_TX_LBL_ENABLE ds_abs1) ==>
+(ref_rel ds_abs1 (dr, spi)) /\ (ABS1_TX_LBL_ENABLE ds_abs1) ==>
 ?dr' spi'. (local_tr (dr, spi) (TX (abs1_tx_trans_done_op_value ds_abs1)) (dr', spi')) /\
-(ref_rel (abs1_tx_trans_done_op_state ds_abs1) dr' spi')``,
+(ref_rel (abs1_tx_trans_done_op_state ds_abs1) (dr', spi'))``,
 rw [local_tr_cases, spi_tr_cases] >|
 [`spi.state = tx_trans_done \/ spi.state = tx_trans_next` 
 by METIS_TAC[ABS1_TX_LBL_ENABLE_def, ref_rel_def, IS_STATE_REL_def] >>
@@ -92,11 +92,12 @@ tx_TX_op_state_def, tx_TX_op_def, tx_trans_next_op_def] >>
 FULL_SIMP_TAC std_ss [ref_rel_def, IS_STATE_REL_def] >>
 rw []]]);
 
+
 (* a lemma for RX label proof *)
 (* If spi.state = rx_receive_data, then abs1 is able to process RX label as well. *)
 val spi_rx_receive_data_imply_abs1_rx_enable = store_thm("spi_rx_receive_data_imply_abs1_rx_enable",
 ``!(spi:spi_state) (dr:driver_state) (ds_abs1:ds_abs1_state).
-(ref_rel ds_abs1 dr spi) /\ (spi.state = rx_receive_data) ==>
+(ref_rel ds_abs1 (dr, spi)) /\ (spi.state = rx_receive_data) ==>
 ABS1_RX_LBL_ENABLE ds_abs1``,
 rw [ABS1_RX_LBL_ENABLE_def] >>
 `IS_STATE_REL ds_abs1 dr spi` by METIS_TAC[ref_rel_def] >>
@@ -108,12 +109,12 @@ rw [] >>
 Cases_on `spi.state` >>
 rw []);
 
-
-(* bisimulation: ds_abs1' exists for RX label *)
-val abs1_comb_hold_ref_rel_RX = store_thm("abs1_comb_hold_ref_rel_RX",
+(* ds_abs1' exists for RX label *)
+val comb_abs1_hold_ref_rel_RX = store_thm("comb_abs1_hold_ref_rel_RX",
 ``!(spi:spi_state) (dr:driver_state) (ds_abs1:ds_abs1_state) (data:word8 option) (spi':spi_state).
-(ref_rel ds_abs1 dr spi) /\ (spi_tr spi (RX data) spi') ==>
-?ds_abs1'. (ds_abs1_tr ds_abs1 (RX data) ds_abs1') /\ (ref_rel ds_abs1' dr spi')``,
+(ref_rel ds_abs1 (dr, spi)) /\ (spi_tr spi (RX data) spi') ==>
+?ds_abs1'. (ds_abs1_tr ds_abs1 (RX data) ds_abs1') /\ 
+(ref_rel ds_abs1' (dr, spi'))``,
 rw [spi_tr_cases, ds_abs1_tr_cases] >|
 [METIS_TAC [spi_rx_receive_data_imply_abs1_rx_enable],
 `ABS1_RX_LBL_ENABLE ds_abs1` by METIS_TAC [spi_rx_receive_data_imply_abs1_rx_enable] >>
@@ -123,13 +124,13 @@ abs1_rx_fetch_data_op_def] >>
 FULL_SIMP_TAC (std_ss++WORD_ss) [ref_rel_def, IS_STATE_REL_def] >>
 rw []]);
 
-(* bisimulation: (dr',spi') exists for RX label *)
-val comb_abs1_hold_ref_rel_RX = store_thm("comb_abs1_hold_ref_rel_RX",
+(* (dr',spi') exists for RX label *)
+val abs1_comb_hold_ref_rel_RX = store_thm("abs1_comb_hold_ref_rel_RX",
 ``!(spi:spi_state) (dr:driver_state) (ds_abs1:ds_abs1_state) (data:word8 option).
-(ref_rel ds_abs1 dr spi) /\ (ABS1_RX_LBL_ENABLE ds_abs1) /\
+(ref_rel ds_abs1 (dr, spi)) /\ (ABS1_RX_LBL_ENABLE ds_abs1) /\
 (data <> NONE) ==>
 ?dr' spi'. local_tr (dr,spi) (RX data) (dr', spi') /\
-(ref_rel (abs1_rx_receive_data_op ds_abs1 data) dr' spi')``,
+(ref_rel (abs1_rx_receive_data_op ds_abs1 data) (dr', spi'))``,
 rw [local_tr_cases, spi_tr_cases] >|
 [METIS_TAC [ref_rel_def, IS_STATE_REL_def, ABS1_RX_LBL_ENABLE_def],
 `spi.state = rx_receive_data` by METIS_TAC[ref_rel_def, IS_STATE_REL_def, ABS1_RX_LBL_ENABLE_def] >>
@@ -139,11 +140,12 @@ abs1_rx_fetch_data_op_def, rx_receive_data_op_def] >>
 FULL_SIMP_TAC std_ss [ref_rel_def, IS_STATE_REL_def] >>
 rw []]);
 
+
 (* a lemma for XFER label *)
 (* If spi.state = xfer_exchange_data, then abs1.state = abs1_xfer_exchange_data *)
 val spi_xfer_exchange_data_imply_abs1_xfer_enable = store_thm("spi_xfer_exchange_data_imply_abs1_xfer_eanble",
 ``!(spi:spi_state) (dr:driver_state) (ds_abs1:ds_abs1_state).
-(ref_rel ds_abs1 dr spi) /\ (spi.state = xfer_exchange_data) ==>
+(ref_rel ds_abs1 (dr, spi)) /\ (spi.state = xfer_exchange_data) ==>
 ds_abs1.state = abs1_xfer_exchange``,
 rw [] >>
 `IS_STATE_REL ds_abs1 dr spi` by METIS_TAC[ref_rel_def] >>
@@ -155,11 +157,12 @@ rw [] >>
 Cases_on `spi.state` >>
 rw []);
 
-(* bisimulation: ds_abs1' holds for XFER label *)
-val abs1_comb_hold_ref_rel_XFER = store_thm("abs1_comb_hold_ref_rel_XFER",
+(* ds_abs1' holds for XFER label *)
+val comb_abs1_hold_ref_rel_XFER = store_thm("comb_abs1_hold_ref_rel_XFER",
 ``!(spi:spi_state) (dr:driver_state) (ds_abs1:ds_abs1_state) (dataIN:word8 option) (dataOUT:word8 option) (spi':spi_state).
-(ref_rel ds_abs1 dr spi) /\ (spi_tr spi (XFER dataIN dataOUT) spi') ==>
-?ds_abs1'. (ds_abs1_tr ds_abs1 (XFER dataIN dataOUT) ds_abs1') /\ (ref_rel ds_abs1' dr spi')``,
+(ref_rel ds_abs1 (dr, spi)) /\ (spi_tr spi (XFER dataIN dataOUT) spi') ==>
+?ds_abs1'. (ds_abs1_tr ds_abs1 (XFER dataIN dataOUT) ds_abs1') /\ 
+(ref_rel ds_abs1' (dr, spi'))``,
 rw [spi_tr_cases] >>
 `ds_abs1.state = abs1_xfer_exchange` by METIS_TAC[spi_xfer_exchange_data_imply_abs1_xfer_enable] >>
 rw [ds_abs1_tr_cases] >|
@@ -173,14 +176,14 @@ abs1_xfer_exchange_op_state_def, abs1_xfer_exchange_op_def] >>
 FULL_SIMP_TAC std_ss [ref_rel_def, IS_STATE_REL_def] >>
 rw []]);
 
-(* bisimulation: (dr',spi') exists for XFER label *)
-val comb_abs1_hold_ref_rel_XFER = store_thm("comb_abs1_hold_ref_rel_XFER",
+(* (dr',spi') exists for XFER label *)
+val abs1_comb_hold_ref_rel_XFER = store_thm("abs1_comb_hold_ref_rel_XFER",
 ``!(spi:spi_state) (dr:driver_state) (ds_abs1:ds_abs1_state) (dataIN:word8 option).
-(ref_rel ds_abs1 dr spi) /\ (ds_abs1.state = abs1_xfer_exchange) /\
+(ref_rel ds_abs1 (dr, spi)) /\ (ds_abs1.state = abs1_xfer_exchange) /\
 (dataIN <> NONE) ==>
 ?dr' spi'. (local_tr (dr, spi) (XFER dataIN (abs1_xfer_exchange_op_value 
 ds_abs1 dataIN)) (dr', spi')) /\ 
-(ref_rel (abs1_xfer_exchange_op_state ds_abs1 dataIN) dr' spi')``,
+(ref_rel (abs1_xfer_exchange_op_state ds_abs1 dataIN) (dr', spi'))``,
 rw [local_tr_cases, spi_tr_cases] >|
 [`spi.state = xfer_exchange_data` by METIS_TAC[ref_rel_def, IS_STATE_REL_def] >>
 rw [abs1_xfer_exchange_op_value_def, abs1_xfer_exchange_op_def,
